{
 "cells": [
  {
   "cell_type": "markdown",
   "metadata": {},
   "source": [
    "# Maths notes for solving the system\n",
    "\n",
    "## These are great notes for understanding the master equation approach but unfortunately the combinatorics of the state space make the problem intractable numerically through the RMT approach... :( stochastic simulations still work of course!\n",
    "\n",
    "### Single serotype model\n",
    "\n",
    "Start with the equivalent master equation for a single serotype system\n",
    "\n",
    "$$P(x,n,t+\\delta t) = \\delta t\\tilde{\\mu}(n)(x+1)P(x+1,n,t) + \\delta t\\tilde{\\Lambda}(n-1)[1-(x-1)]P(x-1,n-1,t) + \\{ 1-\\delta t\\tilde{\\mu}(n)x-\\delta t\\tilde{\\Lambda}(n)(1-x) \\}P(x,n,t)$$\n",
    "\n",
    "$$\\Rightarrow \\,\\, \\frac{{\\rm d}}{{\\rm d}t}P(x,n,t) = \\tilde{\\mu}(n)(x+1)P(x+1,n,t) + \\tilde{\\Lambda}(n-1)[1-(x-1)]P(x-1,n-1,t) -\\tilde{\\mu}(n)xP(x,n,t) - \\tilde{\\Lambda}(n)(1-x) P(x,n,t)$$\n",
    "\n",
    "$$p(n,t) = \\sum_{x=\\{0,1\\}}xP(x,n,t) = P(1,n,t) = 1-P(0,n,t)$$\n",
    "\n",
    "$$\\Rightarrow \\,\\, \\frac{{\\rm d}}{{\\rm d}t}p(n,t) = \\tilde{\\Lambda}(n-1)[1-p(n-1,t)] -\\tilde{\\mu}(n)p(n,t)$$\n",
    "\n",
    "$${\\sf p}(t) \\equiv \\begin{pmatrix} p(0,t) \\\\ p(1,t) \\\\ \\vdots \\end{pmatrix}$$\n",
    "\n",
    "$$\\Rightarrow \\,\\, \\frac{{\\rm d}}{{\\rm d}t}{\\sf p}(t) = -{\\sf A} \\, {\\sf p}(t) + {\\sf b} = -{\\sf A}[{\\sf p}(t)-{\\sf p}_{\\rm eq}]$$\n",
    "\n",
    "$$\\Rightarrow \\,\\, {\\sf p}_{\\rm eq} = {\\sf A}^{-1}{\\sf b}$$\n",
    "\n",
    "$${\\sf A} \\equiv \\begin{pmatrix} \\tilde{\\mu}(0) & 0 & 0 & \\dots \\\\ \\tilde{\\Lambda}(0) & \\tilde{\\mu}(1) & 0 & \\dots \\\\ 0 & \\tilde{\\Lambda}(1) & \\tilde{\\mu}(2) & \\dots \\\\ \\vdots & \\vdots & \\vdots & \\ddots \\end{pmatrix} \\,, \\qquad {\\sf b} \\equiv \\begin{pmatrix} \\tilde{\\Lambda}(0) \\\\ \\tilde{\\Lambda}(1) \\\\ \\vdots \\end{pmatrix} \\,.$$\n",
    "\n",
    "$$\\Rightarrow \\,\\, {\\sf p}(t) = p_{\\rm eq} + [{\\sf p}(t_0)-p_{\\rm eq}]e^{-{\\sf A}(t-t_0)}\\,.$$"
   ]
  },
  {
   "cell_type": "markdown",
   "metadata": {},
   "source": [
    "### Multi-serotype model\n",
    "\n",
    "Remember now that we have defined\n",
    "\n",
    "$\\tilde{\\mu} (\\vert n \\vert ) = \\mu_i \\exp ( \\sigma \\vert n \\vert )$\n",
    "\n",
    "$\\tilde{\\Lambda} (n_i ) = \\Lambda_i \\exp ( -\\epsilon n_i )\\,.$\n",
    "\n",
    "Important to also note here that our notation $\\vert n\\vert$ denotes the $L_1$ norm, i.e., $\\vert n\\vert = \\sum_{\\forall i}n_i$. The new master equation is...\n",
    "\n",
    "$P(\\dots , x_i,\\dots ,n_i,\\dots ,t+\\delta t) =$\n",
    "\n",
    "$\\delta t\\sum_{\\forall i}\\tilde{\\mu}_i( \\vert n\\vert )(x_i+1)P(\\dots , x_i+1,\\dots ,n_i,\\dots ,t)  $ \n",
    "\n",
    "$+ \\delta t\\sum_{\\forall i}\\tilde{\\Lambda}_i(n_i-1)\\big[ 1-(x_i-1)-\\sum_{\\forall i'\\neq i}x_{i'}\\big]P(\\dots , x_i-1,\\dots ,n_i-1,\\dots ,t) $\n",
    "\n",
    "$+ \\delta t\\sum_{\\forall i}\\sum_{\\forall i'}f_{i'i}\\tilde{\\Lambda}_i (n_i-1)(x_{i'}+1)P(\\dots , x_{i'}+1, x_i-1,\\dots ,n_{i'}, n_i-1,\\dots ,t)$\n",
    "\n",
    "$+ \\delta t\\sum_{\\forall i}\\sum_{\\forall i'}f_{ii'}\\tilde{\\Lambda}_{i'} (n_{i'}-1)(x_{i}+1)P(\\dots , x_{i'}-1, x_{i}+1,\\dots ,n_{i'}-1, n_{i},\\dots ,t)$\n",
    "\n",
    "$+ \\big[ 1-\\delta t\\sum_{\\forall i}\\tilde{\\mu}_i( \\vert n\\vert )x_i - \\delta t\\sum_{\\forall i}\\tilde{\\Lambda}_i(n_i)(1-\\sum_{\\forall i'}x_{i'}) - \\delta t\\sum_{\\forall i}\\sum_{\\forall i'}f_{i'i}\\tilde{\\Lambda}_i (n_i)x_{i'} - \\delta t\\sum_{\\forall i}\\sum_{\\forall i'}f_{ii'}\\tilde{\\Lambda}_{i'} (n_{i'})x_{i} \\big] P(\\dots , x_i,\\dots ,n_i,\\dots ,t) \\,.$\n",
    "\n",
    "This gives...\n",
    "\n",
    "$\\frac{{\\rm d}}{{\\rm d}t}P(\\dots , x_i,\\dots ,n_i,\\dots ,t) =$\n",
    "\n",
    "$\\sum_{\\forall i}\\tilde{\\mu}_i( \\vert n\\vert )(x_i+1)P(\\dots , x_i+1,\\dots ,n_i,\\dots ,t)  $ \n",
    "\n",
    "$+ \\sum_{\\forall i}\\tilde{\\Lambda}_i(n_i-1)\\big[ 1-(x_i-1)-\\sum_{\\forall i'\\neq i}x_{i'}\\big]P(\\dots , x_i-1,\\dots ,n_i-1,\\dots ,t) $\n",
    "\n",
    "$+ \\sum_{\\forall i}\\sum_{\\forall i'}f_{i'i}\\tilde{\\Lambda}_i (n_i-1)(x_{i'}+1)P(\\dots , x_{i'}+1, x_i-1,\\dots ,n_{i'}, n_i-1,\\dots ,t)$\n",
    "\n",
    "$+ \\sum_{\\forall i}\\sum_{\\forall i'}f_{ii'}\\tilde{\\Lambda}_{i'} (n_{i'}-1)(x_{i}+1)P(\\dots , x_{i'}-1, x_{i}+1,\\dots ,n_{i'}-1, n_{i},\\dots ,t)$\n",
    "\n",
    "$-\\big[ \\sum_{\\forall i}\\tilde{\\mu}_i( \\vert n\\vert )x_i + \\sum_{\\forall i}\\tilde{\\Lambda}_i(n_i)(1-\\sum_{\\forall i'}x_{i'}) + \\sum_{\\forall i}\\sum_{\\forall i'}f_{i'i}\\tilde{\\Lambda}_i (n_i)x_{i'} + \\sum_{\\forall i}\\sum_{\\forall i'}f_{ii'}\\tilde{\\Lambda}_{i'} (n_{i'})x_{i} \\big] P(\\dots , x_i,\\dots ,n_i,\\dots ,t) \\,.$\n",
    "\n",
    "Let's have a look at...\n",
    "\n",
    "$p_i(\\dots ,n_i,\\dots ,t)\\equiv \\sum_{x_i=\\{0,1\\}}x_iP(\\dots , x_{i},\\dots ,n_{i},\\dots ,t) = P(\\dots , x_{i}=1,\\dots ,n_{i},\\dots ,t)\\,,$\n",
    "\n",
    "where the subscript $x_i=\\{0,1\\}$ denotes summing over the joint $x_i=1 \\cap x_{i'}=0\\,, \\, \\forall i'\\neq i$ state and all of the other joint states where $x_i=0$ (in the latter case for all of these other states the summand is of course zero). This gives and interacting theory of matrices of the form\n",
    "\n",
    "$\\frac{{\\rm d}}{{\\rm d}t}p_i(\\dots ,n_i,\\dots ,t) = \\tilde{\\Lambda}_i(n_i-1)\\big[ 1-p_{i}(\\dots ,n_{i}-1,\\dots ,t)-\\sum_{\\forall i'\\neq i}p_{i'}(\\dots ,n_{i'},\\dots ,t)\\big] $\n",
    "\n",
    "$\\qquad \\qquad \\qquad \\quad + \\sum_{\\forall i'}f_{i'i}\\tilde{\\Lambda}_i (n_i-1)p_{i'}(\\dots ,n_{i'}, n_i-1,\\dots ,t) $\n",
    "\n",
    "$\\qquad \\qquad \\qquad \\quad -\\big[ \\tilde{\\mu}_i( \\vert n\\vert ) + \\sum_{\\forall i'}f_{ii'}\\tilde{\\Lambda}_{i'} (n_{i'}) \\big] p_i(\\dots ,n_i,\\dots ,t) \\,.$"
   ]
  },
  {
   "cell_type": "markdown",
   "metadata": {},
   "source": [
    "### An operator formalism for the multi-serotype model\n",
    "\n",
    "Let's now see if we can construct a Hamiltonian using the multipartite entangled state space system $\\vert {\\sf P}(t)\\rangle =\\sum_{\\forall i}\\sum_{x_i=\\{ 0,1\\}}\\sum_{n_i=0}^\\infty P(\\dots , x_i,\\dots ,n_i,\\dots ,t)\\vert \\dots , x_i, \\dots, n_i,\\dots \\rangle$ and ladder operators for each $\\hat{a}^\\dagger_i,\\hat{a}_i$ and $\\hat{b}^\\dagger_i,\\hat{b}_i$. These operators act on the state space in the following manner\n",
    "\n",
    "$\\hat{a}^\\dagger_i \\vert \\dots , x_i,\\dots \\rangle = \\vert \\dots , x_i+1,\\dots \\rangle$\n",
    "\n",
    "$\\hat{a}_i \\vert \\dots , x_i,\\dots \\rangle = x_i\\vert \\dots , x_i-1,\\dots \\rangle$\n",
    "\n",
    "$\\hat{b}^\\dagger_i \\vert \\dots , n_i,\\dots \\rangle = \\vert \\dots , n_i+1,\\dots \\rangle$\n",
    "\n",
    "$\\hat{b}_i \\vert \\dots , n_i,\\dots \\rangle = n_i\\vert \\dots , n_i-1,\\dots \\rangle$\n",
    "\n",
    "$\\Rightarrow \\,\\, \\hat{a}^\\dagger_i\\hat{a}_i\\vert \\dots , x_i,\\dots \\rangle = x_i\\vert \\dots , x_i,\\dots \\rangle$\n",
    "\n",
    "$\\Rightarrow \\,\\, (\\sum_{\\forall i}\\hat{a}^\\dagger_i\\hat{a}_i)\\vert \\dots , x_i,\\dots \\rangle = (\\sum_{\\forall i}x_i)\\vert \\dots , x_i,\\dots \\rangle$\n",
    "\n",
    "$\\Rightarrow \\,\\, \\hat{b}^\\dagger_i\\hat{b}_i\\vert \\dots , n_i,\\dots \\rangle = n_i\\vert \\dots , n_i,\\dots \\rangle$\n",
    "\n",
    "$\\Rightarrow \\,\\, (\\sum_{\\forall i}\\hat{b}^\\dagger_i\\hat{b}_i)\\vert \\dots , n_i,\\dots \\rangle = (\\sum_{\\forall i}n_i)\\vert \\dots , n_i,\\dots \\rangle$\n",
    "\n",
    "$\\Rightarrow [\\hat{a}_i,\\hat{a}^\\dagger_{i'} ] = \\delta_{ii'}$\n",
    "\n",
    "$\\Rightarrow [\\hat{b}_i,\\hat{b}^\\dagger_{i'} ] = \\delta_{ii'}$\n",
    "\n",
    "All other commutators are $0$...\n",
    "\n",
    "Using these operators, the Hamiltonian is constructed from the following terms. The recovery term of the master equation turns into\n",
    "\n",
    "$\\sum_{\\forall i}\\sum_{x_i=\\{ 0,1\\}}\\sum_{n_i=0}^\\infty\\sum_{\\forall i'}\\tilde{\\mu}_{i'}( \\vert n\\vert )(x_{i'}+1)P(\\dots , x_{i'}+1, x_i,\\dots ,n_{i'},n_i,\\dots ,t) \\vert \\dots , x_{i'}, x_i, \\dots, n_{i'}, n_i,\\dots \\rangle =$\n",
    "\n",
    "$\\sum_{\\forall i}\\sum_{x_i=\\{ 0,1\\}}\\sum_{n_i=0}^\\infty\\sum_{\\forall i'}\\mu_{i'}\\exp (\\sigma \\sum_{\\forall i''} n_{i''}) x_{i'}P(\\dots , x_{i'}, x_i,\\dots ,n_{i'},n_i,\\dots ,t) \\vert \\dots , x_{i'}-1, x_i,\\dots, n_{i'}, n_i,\\dots \\rangle =$\n",
    "\n",
    "$\\sum_{\\forall i'}\\mu_{i'}\\exp \\big( \\sigma \\sum_{\\forall i}\\hat{b}^\\dagger_i\\hat{b}_i\\big) \\hat{a}_{i'} \\vert {\\sf P}(t)\\rangle\\,.$\n",
    "\n",
    "The colonisation term of the master equation turns into \n",
    "\n",
    "$\\sum_{\\forall i}\\sum_{x_i=\\{ 0,1\\}}\\sum_{n_i=0}^\\infty \\sum_{\\forall i'}\\tilde{\\Lambda}_{i'}(n_{i'}-1)\\big[ 1-(x_{i'}-1)-\\sum_{\\forall i''\\neq i'}x_{i''}\\big]P(\\dots , x_{i'}-1,\\dots ,n_{i'}-1,\\dots ,t) \\vert \\dots , x_{i'},x_i,\\dots,n_{i'},n_i,\\dots \\rangle = $\n",
    "\n",
    "$\\sum_{\\forall i}\\sum_{x_i=\\{ 0,1\\}}\\sum_{n_i=0}^\\infty \\sum_{\\forall i'}\\Lambda_{i'} \\exp ( -\\epsilon n_{i'} )\\big[ 1-\\sum_{\\forall i''}x_{i''}\\big]P(\\dots , x_{i'},\\dots ,n_{i'},\\dots ,t) \\vert \\dots , x_{i'}+1,x_i,\\dots \\dots,n_{i'}+1,n_i,\\dots \\rangle =$\n",
    "\n",
    "$\\sum_{\\forall i'}\\Lambda_{i'} \\hat{b}^\\dagger_{i'}\\exp \\big( -\\epsilon \\hat{b}^\\dagger_{i'}\\hat{b}_{i'} \\big) \\hat{a}^\\dagger_{i'}\\big( 1- \\sum_{\\forall i}\\hat{a}^\\dagger_{i}\\hat{a}_{i}\\big) \\vert {\\sf P}(t)\\rangle\\,.$\n",
    "\n",
    "The replacement terms turn into\n",
    "\n",
    "$\\sum_{\\forall i}\\sum_{x_i=\\{ 0,1\\}}\\sum_{n_i=0}^\\infty \\sum_{\\forall i'}\\sum_{\\forall i''}f_{i''i'}\\tilde{\\Lambda}_{i'} (n_{i'}-1)(x_{i''}+1)P(\\dots , x_{i''}+1, x_{i'}-1,\\dots ,n_{i''}, n_{i'}-1,\\dots ,t) \\vert \\dots , x_{i''}, x_{i'}, x_i,\\dots , n_{i''}, n_{i'},n_i,\\dots \\rangle =$\n",
    "\n",
    "$\\sum_{\\forall i}\\sum_{x_i=\\{ 0,1\\}}\\sum_{n_i=0}^\\infty \\sum_{\\forall i'}\\sum_{\\forall i''}f_{i''i'}\\tilde{\\Lambda}_{i'} (n_{i'})x_{i''}P(\\dots , x_{i''}, x_{i'},\\dots ,n_{i''}, n_{i'},\\dots ,t) \\vert \\dots , x_{i''}-1, x_{i'}+1, x_i,\\dots , n_{i''}, n_{i'}+1,n_i,\\dots \\rangle =$\n",
    "\n",
    "$\\sum_{\\forall i'}\\sum_{\\forall i''}f_{i''i'}\\Lambda_{i'} \\hat{b}^\\dagger_{i'}\\exp \\big( -\\epsilon \\hat{b}^\\dagger_{i'}\\hat{b}_{i'} \\big) \\hat{a}^\\dagger_{i'}\\hat{a}_{i''} \\vert {\\sf P}(t)\\rangle\\,.$\n",
    "\n",
    "...and...\n",
    "\n",
    "$\\sum_{\\forall i}\\sum_{x_i=\\{ 0,1\\}}\\sum_{n_i=0}^\\infty \\sum_{\\forall i'}\\sum_{\\forall i''}f_{i'i''}\\tilde{\\Lambda}_{i''} (n_{i''}-1)(x_{i'}+1)P(\\dots , x_{i''}-1, x_{i'}+1,\\dots ,n_{i''}-1, n_{i'},\\dots ,t) \\vert \\dots , x_{i''}, x_{i'}, x_i, \\dots, n_{i''}, n_{i'},n_i,\\dots \\rangle =$\n",
    "\n",
    "$\\sum_{\\forall i}\\sum_{x_i=\\{ 0,1\\}}\\sum_{n_i=0}^\\infty \\sum_{\\forall i'}\\sum_{\\forall i''}f_{i'i''}\\tilde{\\Lambda}_{i''} (n_{i''})x_{i'}P(\\dots , x_{i''}, x_{i'},\\dots ,n_{i''}, n_{i'},\\dots ,t) \\vert \\dots , x_{i''}+1, x_{i'}-1, x_i, \\dots, n_{i''}+1, n_{i'},n_i,\\dots \\rangle =$\n",
    "\n",
    "$\\sum_{\\forall i'}\\sum_{\\forall i''}f_{i'i''}\\Lambda_{i''} \\hat{b}^\\dagger_{i''}\\exp \\big( -\\epsilon \\hat{b}^\\dagger_{i''}\\hat{b}_{i''} \\big) \\hat{a}^\\dagger_{i''}\\hat{a}_{i'} \\vert {\\sf P}(t)\\rangle\\,.$\n",
    "\n",
    "Lastly, the 'do nothing' (or rejection) term turns into\n",
    "\n",
    "$\\sum_{\\forall i}\\sum_{x_i=\\{ 0,1\\}}\\sum_{n_i=0}^\\infty\\big[ \\sum_{\\forall i'}\\tilde{\\mu}_{i'}( \\vert n\\vert )x_{i'} + \\sum_{\\forall i'}\\tilde{\\Lambda}_{i'}(n_{i'})(1-\\sum_{\\forall i''}x_{i''}) + \\sum_{\\forall i'}\\sum_{\\forall i''}f_{i''i'}\\tilde{\\Lambda}_{i'} (n_{i'})x_{i''} + \\sum_{\\forall i'}\\sum_{\\forall i''}f_{i'i''}\\tilde{\\Lambda}_{i''} (n_{i''})x_{i'} \\big] P(\\dots , x_{i'},\\dots ,n_{i'},\\dots ,t) \\vert \\dots , x_{i'}, x_i, \\dots, n_{i'}, n_i,\\dots \\rangle =$\n",
    "\n",
    "$\\big[ \\sum_{\\forall i'}\\mu_{i'}\\exp \\big( \\sigma \\sum_{\\forall i}\\hat{b}^\\dagger_i\\hat{b}_i\\big) \\hat{a}^\\dagger_{i'}\\hat{a}_{i'} + \\sum_{\\forall i'}\\Lambda_{i'} \\exp \\big( -\\epsilon \\hat{b}^\\dagger_{i'}\\hat{b}_{i'} \\big) \\big( 1- \\sum_{\\forall i}\\hat{a}^\\dagger_{i}\\hat{a}_{i}\\big) +\\sum_{\\forall i'}\\sum_{\\forall i''}f_{i''i'}\\Lambda_{i'} \\exp \\big( -\\epsilon \\hat{b}^\\dagger_{i'}\\hat{b}_{i'} \\big) \\hat{a}^\\dagger_{i''}\\hat{a}_{i''} + \\sum_{\\forall i'}\\sum_{\\forall i''}f_{i'i''}\\Lambda_{i''} \\exp \\big( -\\epsilon \\hat{b}^\\dagger_{i''}\\hat{b}_{i''} \\big) \\hat{a}^\\dagger_{i'}\\hat{a}_{i'} \\big] \\vert {\\sf P}(t)\\rangle\\,.$\n",
    "\n",
    "We therefore have...\n",
    "\n",
    "$\\frac{{\\rm d}}{{\\rm d}t}\\vert {\\sf P}(t)\\rangle = \\hat{{\\cal H}}\\vert {\\sf P}(t)\\rangle$\n",
    "\n",
    "$\\Rightarrow \\,\\, \\vert {\\sf P}(t)\\rangle = e^{\\hat{{\\cal H}}(t-t_0)}\\vert {\\sf P}(t_0)\\rangle$\n",
    "\n",
    "$\\hat{{\\cal H}} = \\sum_{\\forall i'}\\mu_{i'}(1-\\hat{a}^\\dagger_{i'})\\exp \\big( \\sigma \\sum_{\\forall i}\\hat{b}^\\dagger_i\\hat{b}_i\\big) \\hat{a}_{i'} + \\sum_{\\forall i'}\\Lambda_{i'} (\\hat{b}^\\dagger_{i'}\\hat{a}^\\dagger_{i'} - 1)\\exp \\big( -\\epsilon \\hat{b}^\\dagger_{i'}\\hat{b}_{i'} \\big) \\big( 1- \\sum_{\\forall i}\\hat{a}^\\dagger_{i}\\hat{a}_{i}\\big) $\n",
    "\n",
    "$\\qquad + 2\\sum_{\\forall i'}\\sum_{\\forall i''}f_{i''i'}\\Lambda_{i'} \\hat{b}^\\dagger_{i'}\\exp \\big( -\\epsilon \\hat{b}^\\dagger_{i'}\\hat{b}_{i'} \\big) (\\hat{a}^\\dagger_{i'}-\\hat{a}^\\dagger_{i''})\\hat{a}_{i''}  \\,.$\n",
    "\n",
    "The matrix representations of these operators in the Hamiltonian can be generated through ${\\cal O}_{i'i}(t) = \\langle {\\sf p}_{i'}(t)\\vert \\hat{{\\cal O}}\\vert {\\sf p}_i(t)\\rangle$, i.e., the all-zero state would be $\\langle \\dots , 0 , \\dots , 0  , \\dots  \\vert \\hat{{\\cal O}}\\vert \\dots , 0 , \\dots , 0  , \\dots  \\rangle$. **Note that with $N_{\\rm s}$ serotypes and $N_{\\rm c}$ maximum possible carriages over lifetime, the state space combinatorics are crazy: $(N_{\\rm s}+1)(N_{\\rm c}+1)^{N_{\\rm s}+1}$ so when we simulate the system we will have to truncate the state space at relatively low values.**\n",
    "\n",
    "The solution on a finite state space becomes\n",
    "\n",
    "$\\frac{{\\rm d}}{{\\rm d}t}{\\sf p}_{ij}(t) = \\frac{{\\rm d}}{{\\rm d}t}\\langle {\\sf p}_i(t) \\vert {\\sf p}_j(t)\\rangle = \\langle {\\sf p}_i(t) \\vert \\hat{{\\cal H}} \\vert {\\sf p}_j(t)\\rangle = \\sum_{\\forall i'} \\langle {\\sf p}_i(t) \\vert \\hat{{\\cal H}} \\vert {\\sf p}_{i'}(t) \\rangle \\langle {\\sf p}_{i'}(t)\\vert {\\sf p}_j(t)\\rangle =\\sum_{\\forall i'}{\\cal H}_{ii'}{\\sf p}_{i'j}(t)$\n",
    "\n",
    "${\\sf p}_{ij}(t) = \\sum_{\\forall i'} \\big[ e^{{\\cal H}(t-t_0)} \\big]_{ii'}{\\sf p}_{i'j}(t_0)\\,,$\n",
    "\n",
    "where we could use the equation above to initialise a pure ensemble in the $j$-th state such that ${\\sf p}_{i'j}(t_0) = \\delta_{i'j}$.\n",
    "\n",
    "The adjoint equation is\n",
    "\n",
    "$\\frac{{\\rm d}}{{\\rm d}t}\\langle {\\sf P}(t)\\vert = \\langle {\\sf P}(t)\\vert \\hat{{\\cal H}}^\\dagger$\n",
    "\n",
    "$\\hat{{\\cal H}}^\\dagger = \\sum_{\\forall i'}\\mu_{i'}(1-\\hat{a}^\\dagger_{i'}) \\exp \\big( \\sigma \\sum_{\\forall i}\\hat{b}^\\dagger_i\\hat{b}_i\\big) \\hat{a}_{i'} + \\sum_{\\forall i'}\\Lambda_{i'} \\big( 1- \\sum_{\\forall i}\\hat{a}^\\dagger_{i}\\hat{a}_{i}\\big) \\exp \\big( -\\epsilon \\hat{b}^\\dagger_{i'}\\hat{b}_{i'} \\big) (\\hat{a}_{i'}\\hat{b}_{i'} - 1)$\n",
    "\n",
    "$\\qquad + 2\\sum_{\\forall i'}\\sum_{\\forall i''}f_{i''i'}\\Lambda_{i'} \\hat{a}^\\dagger_{i''} (\\hat{a}_{i'}-\\hat{a}_{i''})  \\exp \\big( -\\epsilon \\hat{b}^\\dagger_{i'}\\hat{b}_{i'} \\big)  \\hat{b}_{i'} \\,.$\n",
    "\n",
    "**Note that this system is non-Hermitian which is ok but unusual! Look into non-Hermitian systems - these are typically dissipative systems which are far from equilibrium - https://arxiv.org/abs/1904.13082 -  https://en.wikipedia.org/wiki/Non-Hermitian_quantum_mechanics.** To use this equation for investigating how attractive and repulsive states are over time we can write\n",
    "\n",
    "$\\frac{{\\rm d}}{{\\rm d}t}{\\sf p}_{ij}(t) = \\frac{{\\rm d}}{{\\rm d}t}\\langle {\\sf p}_i(t)\\vert {\\sf p}_j(t) \\rangle = \\langle {\\sf p}_{i}(t)\\vert \\hat{{\\cal H}}^\\dagger \\vert {\\sf p}_j(t) \\rangle = \\sum_{\\forall i'}\\langle {\\sf p}_{i}(t)\\vert {\\sf p}_{i'}(t) \\rangle \\langle {\\sf p}_{i'}(t) \\vert \\hat{{\\cal H}}^\\dagger \\vert {\\sf p}_j(t) \\rangle = \\sum_{\\forall i'}{\\sf p}_{ii'}(t) {\\cal H}^\\dagger_{i'j}\\,.$\n",
    "\n",
    "Binding states together in the following way ${\\sf p}^N_{j}(t)=\\sum_{i=1}^N{\\sf p}_{ij}(t)$ and setting all other other states to $0$ as dynamical sinks, the above equation is simply \n",
    "\n",
    "$\\frac{{\\rm d}}{{\\rm d}t}{\\sf p}^N_{j}(t)=\\sum_{\\forall i'}{\\sf p}^N_{i'}(t) {\\cal H}^\\dagger_{i'j} \\,\\, \\Leftrightarrow \\,\\, {\\sf p}^N_{j}(t) = \\sum_{\\forall i'}{\\sf p}^N_{i'}(t_0)\\big[ e^{{\\cal H}^\\dagger (t-t_0)}\\big]_{i'j}\\,.$\n",
    "\n",
    "The retention probability above (and its converse where all other states are non-zero apart from these ones) can be used to investigate the success and/or failure of vaccine strategies etc...\n",
    "\n",
    "**USE RMT TO INVESTIGATE SPECTRAL PROPERTIES OF THE HAMILTONIAN!!! (https://arxiv.org/abs/1904.13082)**"
   ]
  },
  {
   "cell_type": "code",
   "execution_count": null,
   "metadata": {},
   "outputs": [],
   "source": []
  }
 ],
 "metadata": {
  "kernelspec": {
   "display_name": "Python 3",
   "language": "python",
   "name": "python3"
  },
  "language_info": {
   "codemirror_mode": {
    "name": "ipython",
    "version": 3
   },
   "file_extension": ".py",
   "mimetype": "text/x-python",
   "name": "python",
   "nbconvert_exporter": "python",
   "pygments_lexer": "ipython3",
   "version": "3.7.7"
  }
 },
 "nbformat": 4,
 "nbformat_minor": 2
}
